\begin{minted}{haskell}
a 0 m = m+1
a n 0 = a (n-1) 1
a n m = a (n-1) (a n (m-1))
\end{minted}
\begin{minted}{haskell}
alist []     ys     = [1]++ys
alist (x:xs) []     = alist xs [x]
alist (x:xs) (y:ys) = alist xs (alist (x:xs) ys)
\end{minted}
\begin{claim}The following equation holds.
\begin{minted}{haskell}
length (alist xs ys) = a (length xs) (length ys)
\end{minted}
\end{claim}
\begin{align*}
(xs,ys)&\prec(\hphantom{(x:\ }xs\hphantom{)},(y:ys))\\
(xs,zs)&\prec((x:xs),\hphantom{(x:\ }ys\hphantom{)})
\end{align*}
\begin{minted}{haskell}
r []     = []
r (x:xs) = r (xs++[(x+1)]++[(x+1)])
\end{minted}
\begin{claim}The following equation holds.
\begin{minted}{haskell}
r xs = []
\end{minted}
\end{claim}
