\section{Boolean Rings}
\begin{frame}{Boolean Rings}
\[B:=\left\lbrace 
	\begin{aligned}
		x+y     & \approx y+x,         & x*y     & \approx y*x,     \\
		(x+y)+z & \approx x+(y+z),     & (x*y)*z & \approx x*(y*z), \\
		x+x     & \approx 0,           & x*x     & \approx x,       \\
		0+x     & \approx x,           & 0*x     & \approx 0,       \\
		x*(y+z) & \approx (x*y)+(x*z), & 1*x     & \approx x        
	\end{aligned}
	\right\rbrace \]
\end{frame}

\begin{frame}{Boolean Rings}{Interpretation}
$\BTwo:=(\Delta^\BTwo,\cdot^\BTwo)$\\
\vspace{10pt}\hspace{10pt}
$\Delta^\BTwo:=\left\lbrace\bot,\top\right\rbrace$
\uncover<2->{
\begin{align*}
	(x+y)^\BTwo & :=\left( x^\BTwo\wedge\neg y^\BTwo\right)  \vee \left( \neg x^\BTwo\wedge y^\BTwo\right) \\ 
	(x*y)^\BTwo & :=x^\BTwo\wedge y^\BTwo \\
	0^\BTwo     & :=\bot \\ 
	1^\BTwo     & :=\top                  
\end{align*}
}
\end{frame}

\begin{frame}{Boolean Rings}{Example}	
\begin{align*}
	(1+0)^\BTwo&=\left( 1^\BTwo\wedge\neg 0^\BTwo\right) \vee \left( \neg1^\BTwo\wedge 0^\BTwo\right) \\
	&=\left( \top\wedge\neg\bot\right) \vee\left(\neg\top\wedge\bot \right) \\
	&=\top\vee\bot\\
	&=\top
\end{align*}
\end{frame}

\begin{frame}{Boolean Rings}{Polynomial Form}	
\begin{align*}
asd
\end{align*}
\end{frame}
\section{Unification modulo Boolean Rings}