\section{sum prod tails}
\begin{code}
tails :: [a] -> [[a]]
tails []         = [[]]
tails xxs@(_:xs) = xxs:(tails xs)
\end{code}
\begin{code}
sum = foldl + 0
\end{code}
\begin{code}
product = foldl * 1
\end{code}
\begin{claim}\label{tailsClaim}\ 
\begin{code}
sum.map product.tails = foldl f 1
                f x y = x*y+1
\end{code}
\end{claim}\begin{lemma}\label{sumLemma}\ 
\begin{code}
sum (x:ys) = x+(sum ys)
\end{code}
\end{lemma}
\begin{proof} of Lemma \ref{sumLemma} by structural induction on ys\\
\verb|ys=[]|
\begin{code}
\end{code}
\verb|ys=(y:ys')|
\begin{code}
\end{code}
\end{proof}
%-----------------------------------------------------------------------------------
\begin{lemma}\label{prodLemma}\ 
\begin{code}
product (x:ys) = x(product ys)
\end{code}
\end{lemma}
\begin{proof} of Lemma \ref{prodLemma} by structural induction on ys\\
\verb|ys=[]|
\begin{code}
\end{code}
\verb|ys=(y:ys')|
\begin{code}
\end{code}
\end{proof}
%-----------------------------------------------------------------------------------
\begin{lemma}\label{prodfoldlLemma}\ 
\begin{code}
foldl f (x+1) ys = x(product ys) + (foldl f 1 ys)
\end{code}
\end{lemma}
\begin{proof} of Lemma \ref{prodfoldlLemma} by structural induction on ys\\
\verb|ys=[]|
\begin{code}
foldl f (x+1) ys
           = foldl f (x+1) []
           = x+1
           = x(product []) + (foldl f 1 [])
           = x(product ys) + (foldl f 1 ys)
\end{code}
\verb|ys=(y:ys')|
\begin{code}
foldl f (x+1) ys
           = foldl f (x+1) (y:ys')
           = foldl f (f (x+1) y) ys'
           = foldl f (xy+y+1) ys'
           (*\sEq{IH}*) (xy+y)(product ys') + (foldl f 1 ys')
           = xy(product ys') + y(product ys') + (foldl f 1 ys')
           (*\sEq{IH}*) xy(product ys') + (foldl f (y+1) ys')
           = xy(product ys') + (foldl f (f 1 y) ys')
           = xy(product ys') + (foldl f 1 (y:ys'))
           (*\sEq{\ref{prodLemma}}*) x(product (y:ys')) + (foldl f 1 (y:ys'))
           = x(product ys) + (foldl f 1 ys)
\end{code}
\end{proof}
%-----------------------------------------------------------------------------------
\begin{proof} of Claim \ref{tailsClaim}\\
we show the equivalent claim\\
\verb|sum (map product (tails xs)) = foldl f 1 xs|\\
\verb|                       f x y = x*y+1|\\
by structural induction on xs\\
\verb|xs=[]|
\begin{code}
sum (map product (tails xs)) 
              = sum (map product (tails []))
              = sum (map product [[]])
              = sum [product []]
              = sum [1]
              = 1
              = foldl f 1 []
              = foldl f 1 xs
\end{code}
\verb|xs=(x:xs')|
\begin{code}
sum (map product (tails xs)) 
              = sum (map product (tails (x:xs')))
              = sum (map product ((x:xs'):(tails xs')))
              = sum ((product (x:xs')):(map product (tails xs')))
              (*\sEq{\ref{sumLemma}}*) (product (x:xs')) + (sum (map product (tails xs')))
              (*\sEq{IH}*) (product (x:xs')) + (foldl f 1 xs')
              (*\sEq{\ref{prodLemma}}*) x(product xs') + (foldl f 1 xs')
              (*\sEq{\ref{prodfoldlLemma}}*) foldl f (x+1) xs'
              = foldl f (f 1 x) xs'
              = foldl f 1 (x:xs')
              = foldl f 1 xs
\end{code}
\end{proof}