\section{bag}
\begin{code}
data Bag a = ListBag [(a,Integer)] deriving (Eq,Show)
\end{code}
%doch nur add::a->Bag a->Bag a?
\begin{code}
add :: Eq a => (a,Integer) -> (Bag a) -> (Bag a)
add (ele,count) (ListBag bagx)
    |ele 'elem' map fst bagx = ListBag (map (inc (ele,count)) bagx) 
    |otherwise               = ListBag (bagx++[(ele,count)])
\end{code}
\begin{code}
inc :: Eq a => (a,Integer) -> (a,Integer) -> (a,Integer)
inc (e,c) (x,z)
    |e==x    = (e,c+z)
    |othwise = (x,z)
\end{code}
\begin{code}
unite :: Eq a => (Bag a) -> (Bag a) -> (Bag a)
unite (ListBag [])     bagy = bagy
unite (ListBag (x:xs)) bagy = unite (ListBag xs) (add x bagy)
\end{code}
\begin{code}
bag :: Eq a => [a] -> (Bag a)
bag []     = Listbag []
bag (x:xs) = add (x,1) (bag xs)
\end{code}
\begin{claim}\label{bagClaim}\ 
\begin{code}
bag (xs++ys) = unite (bag xs) (bag ys) 
\end{code}
\end{claim}
used but unproven statements:
\begin{code}
S1: map f (xs++ys) = (map f xs)++(map f ys)
S2: map f (map g xs) = map (f.g) xs
\end{code}
%-------------------------------------------------------------------------------
\begin{lemma}\label{sameIncLemma}\ 
\begin{code}
(inc (e,z)).(inc (e,c)) = inc (e,z+c)
\end{code}
\end{lemma}
\begin{proof} of Lemma \ref{sameIncLemma}
Case 1 : \verb|A1: f!=e|
\begin{code}
(inc (e,z)).(inc (e,c)) (f,y) = inc (e,z) ((inc (e,c)) (f,y))
                              (*\sEq{A1}*) inc (e,z) (f,y)
                              (*\sEq{A1}*) (f,y)
                              (*\sEq{A1}*) inc (e,z+c) (f,y)
\end{code}
Case 2 : \verb|A1: f==e|
\begin{code}
(inc (e,z)).(inc (e,c)) (f,z) (*\sEq{A1}*) inc (e,z) ((inc (e,c)) (e,y))
                              = inc (e,z) (e,y+c)
                              = (e,y+c+z)
                              = inc (e,z+c) (f,z)
\end{code}
\end{proof}
%-------------------------------------------------------------------------------
\begin{lemma}\label{swapIncLemma}\ 
\begin{code}
(inc (f,z)).(inc (e,c)) = (inc (e,c)).(inc (f,z))
\end{code}
\end{lemma}
\begin{proof} of Lemma \ref{swapIncLemma}
Case 1 : \verb|A1: g!=e|
\begin{code}
(inc (f,z)).(inc (e,c)) (g,y) = inc (f,z) ((inc (e,c)) (g,y))
                              (*\sEq{A1}*) inc (f,z) (g,y)
\end{code}
Case 1.1 : \verb|A2: g!=f|
\begin{code}
                              (*\sEq{A1}*) inc (f,z) (g,y)
                              (*\sEq{A2}*) (g,y)
                              (*\sEq{A1}*) inc (e,c) (g,y)
                              (*\sEq{A2}*) inc (e,c) ((inc (f,z)) (g,y))
                              = (inc (e,c)).(inc (f,z)) (g,y)
\end{code}
Case 1.2 : \verb|A2: g==f|
\begin{code}
                              (*\sEq{A1}*) inc (f,z) (g,y)
                              (*\sEq{A2}*) inc (f,z) (f,y)
                              = (f,y+z)
                              (*\sEq{A1,A2}*) inc (e,c) (f,y+z)
                              = inc (e,c) ((inc (f,z)) (f,y))
                              (*\sEq{A1}*) (inc (e,c)).(inc (f,z)) (g,y)
\end{code}
Case 2 : \verb|A1: f==e|
\begin{code}
(inc (f,z)).(inc (e,c)) (g,y) (*\sEq{A1}*) inc (f,z) ((inc (e,c)) (e,y))
                              = inc (f,z) (e,c+y)
\end{code}
Case 2.1 : \verb|A2: e!=f|
\begin{code}
                              = inc (f,z) (e,c+y)
                              (*\sEq{A2}*) (e,c+y)
                              = inc (e,c) (e,y)
                              (*\sEq{A2}*) inc (e,c) ((inc (f,z)) (e,y))
                              (*\sEq{A1}*) (inc (e,c)).(inc (f,z)) (g,y)
\end{code}
Case 2.2 : \verb|A2: e==f|
\begin{code}
                              = inc (f,z) (e,c+y)
                              (*\sEq{A2}*) inc (f,z) (f,c+y)
                              = (f,z+c+y)
                              = inc (f,c) (f,y+z)
                              = inc (f,c) ((inc (f,z)) (f,y))
                              (*\sEq{A1,A2}*) (inc (e,c)).(inc (f,z)) (g,y)
\end{code}
\end{proof}
%-------------------------------------------------------------------------------
\begin{lemma}\label{mapLemma}if \verb|A1: not e 'elem' map fst xs| inc does not do anything
\begin{code}
xs = map (inc (e,c)) xs
\end{code}
\end{lemma}
\begin{proof} of Lemma \ref{mapLemma} by structural induction on xs\\
\verb|A1: not e 'elem' map fst xs|\\
\verb|xs=[]|
\begin{code}
xs = []
   = map (inc (e,c)) []
   = map (inc (e,c)) xs
\end{code}
\verb|xs=((f,z):xs')|
\begin{code}
xs = (f,z):xs'
   (*\sEq{IH}*) (f,z):(map (inc (e,c)) xs')
   (*\sEq{A1}*) (inc (e,c) (f,z)):(map (inc (e,c)) xs')
   = map (inc (e,c)) ((f,z):xs')
   = map (inc (e,c)) xs
\end{code}
\end{proof}
%-------------------------------------------------------------------------------
\begin{lemma}\label{addSameLemma} adding same element
\begin{code}
add (e,z) (add (e,c) (ListBag xs)) = add (e,c+z) (ListBag xs)
\end{code}
\end{lemma}
\begin{proof} of Lemma \ref{addSameLemma}\\
Case 1 : \verb|A1: not e 'elem' map fst xs|
\begin{code}
add (e,z) (add (e,c) (ListBag xs)) 
             (*\sEq{A1}*) add (e,z) (ListBag (xs++[(e,c)]))
             = ListBag (map (inc (e,z)) (xs++[(e,c)]))
             (*\sEq{S1}*) ListBag ((map (inc (e,z)) xs)++(map (inc (e,z)) [(e,c)]))
             (*\sEq{\ref{mapLemma},A1}*) ListBag (xs++(map (inc (e,z)) [(e,c)]))
             = ListBag (xs++((inc (e,z) (e,c)):(map (inc (e,z)) [])))
             = ListBag (xs++((inc (e,z) (e,c)):[]))
             = ListBag (xs++((e,z+c):[]))
             = ListBag (xs++[(e,z+c)])
             (*\sEq{A1}*) add (e,c+z) (ListBag xs)
\end{code}
Case 2 : \verb|A1: e 'elem' map fst xs|
\begin{code}
add (e,z) (add (e,c) (ListBag xs)) 
             (*\sEq{A1}*) add (e,z) (ListBag (map (inc (e,c)) xs))
             (*\sEq{A1}*) ListBag (map (inc (e,z)) (map (inc (e,c)) xs))
             (*\sEq{S2}*) ListBag (map (inc (e,z)).(inc (e,c)) xs)
             (*\sEq{\ref{sameIncLemma}}*) ListBag (map (inc (e,c+z)) xs)
             (*\sEq{A1}*) add (e,c+z) (ListBag xs)
\end{code}
\end{proof}
%-------------------------------------------------------------------------------
\begin{lemma}\label{addDiffLemma}adding different elements\\
\verb|A1: e 'elem' map fst xs|\\
\verb|A2: f!=e|
\begin{code}
add (f,z) (add (e,c) (ListBag xs)) = add (e,c) (add (f,z) (ListBag xs))
\end{code}
\end{lemma}
\begin{proof} of Lemma \ref{addDiffLemma}\\
\verb|A1: e 'elem' map fst xs|\\
\verb|A2: f!=e|\\
Case 1 : \verb|A3: not f 'elem' map fst xs|
\begin{code}
add (f,z) (add (e,c) (ListBag xs)) 
             (*\sEq{A1}*) add (f,z) (ListBag (map (inc (e,c)) xs))
             (*\sEq{A3}*) ListBag ((map (inc (e,c)) xs)++[(f,z)])
             (*\sEq{A2}*) ListBag ((map (inc (e,c)) xs)++[inc (e,c) (f,z)])
             = ListBag ((map (inc (e,c)) xs)++(map (inc (e,c)) [(f,z)]))
             (*\sEq{S1}*) ListBag (map (inc (e,c)) (xs++[(f,z)]))
             (*\sEq{A1,A2}*) add (e,c) (ListBag (xs++[(f,z)]))
             (*\sEq{A3}*) add (e,c) (add (f,z) (ListBag xs))
\end{code}
Case 2 : \verb|A3: f 'elem' map fst xs|
\begin{code}
add (f,z) (add (e,c) (ListBag xs)) 
             (*\sEq{A1}*) add (f,z) (ListBag (map (inc (e,c)) xs))
             (*\sEq{A3}*) ListBag (map (inc (f,z)) (map (inc (e,c)) xs))
             (*\sEq{S2}*) ListBag (map (inc (f,z)).(inc (e,c)) xs)
             (*\sEq{\ref{swapIncLemma}}*) ListBag (map (inc (e,c)).(inc (f,z)) xs)
             (*\sEq{S2}*) ListBag (map (inc (e,c)) (map (inc (f,z)) xs))
             (*\sEq{A1}*) add (e,c) (ListBag (map (inc (f,z)) xs))
             (*\sEq{A3}*) add (e,c) (add (f,z) (ListBag xs))
\end{code}
\end{proof}
%-------------------------------------------------------------------------------
\begin{lemma}\label{incLemma}if  \verb|A1: not e 'elem' map fst xs|
\begin{code}
unite (ListBag ((e,c):(xs++[(e,z)]++ys))) bagy 
                 = unite (ListBag ((e,c+z):(xs++ys))) bagy
\end{code}
\end{lemma}
\begin{proof} of Lemma \ref{incLemma} by structural induction on xs\\
\verb|A1: not e 'elem' map fst xs|\\
\verb|xs=[]|
\begin{code}
unite (ListBag ((e,c):(xs++[(e,z)]++ys))) bagy 
                 = unite (ListBag ((e,c):([]++[(e,z)]++ys))) bagy
                 = unite (ListBag ((e,c):([(e,z)]++ys))) bagy
                 = unite (ListBag [(e,z)]++ys) (add (e,c) bagy)
                 = unite (ListBag ys) (add (e,z) (add (e,c) bagy))
                 (*\sEq{\ref{addSameLemma}}*) unite (ListBag ys) (add (e,c+z) bagy)
                 = unite (ListBag ((e,c+z):ys)) bagy
                 = unite (ListBag ((e,c+z):(xs++ys))) bagy
\end{code}
\verb|xs=xs'++[x]|
\begin{code}
unite (ListBag ((e,c):(xs++[(e,z)]++ys))) bagy 
  = unite (ListBag (xs++[(e,z)]++ys)) (add (e,c) bagy)
  = unite (ListBag (xs'++[x]++[(e,z)]++ys)) (add (e,c) bagy)
  = unite (ListBag ys) (add (e,z) (add x (add ... (add (e,c) bagy)...)))
  (*\sEq{\ref{addDiffLemma}}*) unite (ListBag ys) (add x (add (e,z) (add ... (add (e,c) bagy)...)))
  = unite (ListBag (xs'++[(e,z)]++[x]++ys)) (add (e,c) bagy)
  = unite (ListBag ((e,c):(xs'++[(e,z)]++[x]++ys))) bagy
  (*\sEq{IH}*) unite (ListBag ((e,c+z):(xs'++[x]++ys))) bagy
  = unite (ListBag ((e,c+z):(xs++ys))) bagy
\end{code}
\end{proof}
%-------------------------------------------------------------------------------
\begin{lemma}\label{addLemma}\ 
\begin{code}
add (e,z) (unite (ListBag xs) bagy)
                 = unite (add (e,z) (ListBag xs)) bagy
\end{code}
\end{lemma}
\begin{proof} of Lemma \ref{addLemma} by structural induction on xs\\
\verb|xs=[]|
\begin{code}
add (e,z) (unite (ListBag xs) bagy) 
             = add (e,z) (unite (ListBag []) bagy)
             = add (e,z) bagy
             = unite (ListBag []) (add (e,z) bagy)
             = unite (ListBag [(e,z)]) bagy
             = unite (add (e,z) (ListBag [])) bagy
             = unite (add (e,z) (ListBag xs)) bagy
\end{code}
\verb|xs=(x:xs')|
\begin{code}
add (e,z) (unite (ListBag xs) bagy)
             = add (e,z) (unite (ListBag (x:xs')) bagy)
             = add (e,z) (unite (ListBag xs') (add x bagy))
             (*\sEq{IH}*) unite (add (e,z) (ListBag xs')) (add x bagy)
\end{code}
\hspace{1cm}Case 1 : \verb|A1: not e 'elem' map fst xs|
\begin{code}
             (*\sEq{IH}*) unite (add (e,z) (ListBag xs')) (add x bagy)
             (*\sEq{A1}*) unite (ListBag (xs'++[(e,z)])) (add x bagy)
             = unite (ListBag (x:(xs'++[(e,z)]))) bagy
             = unite (ListBag ((x:xs')++[(e,z)])) bagy
             = unite (ListBag (xs++[(e,z)])) bagy
             (*\sEq{A1}*) unite (add (e,z) (ListBag xs)) bagy

\end{code}
\hspace{1cm}Case 2.1 : \verb|A1: e 'elem' map fst xs| and \verb|A2: x=(f,c) f!=e|\\
\hphantom{\hspace{1cm}Case 2.1 : }\verb|A1| and \verb|A2| imply \verb|A3: e 'elem' map fst xs'|
\begin{code}
             (*\sEq{IH}*) unite (add (e,z) (ListBag xs')) (add x bagy)
             (*\sEq{A3}*) unite (ListBag (map (inc (e,z)) xs')) (add x bagy)
             = unite (ListBag (x:(map (inc (e,z)) xs'))) bagy
             (*\sEq{A2}*) unite (ListBag ((inc (e,z) x):(map (inc (e,z)) xs'))) bagy
             = unite (ListBag (map (inc (e,z)) (x:xs'))) bagy
             (*\sEq{A1}*) unite (add (e,z) (ListBag xs)) bagy

\end{code}
\hspace{1cm}Case 2.2 : \verb|A1: e 'elem' map fst xs| and \verb|A2: x=(e,c)|\\
\hphantom{\hspace{1cm}Case 2.2 : }multiset, \verb|A1| and \verb|A2| imply \verb|A3: not e 'elem' map fst xs'|
\begin{code}
             (*\sEq{IH}*) unite (add (e,z) (ListBag xs')) (add x bagy)
             (*\sEq{A3}*) unite (ListBag (xs'++[(e,z)])) (add x bagy)
             = unite (ListBag (x:(xs'++[(e,z)]))) bagy
             (*\sEq{A2}*) unite (ListBag ((e,c):(xs'++[(e,z)]))) bagy
             (*\sEq{\ref{incLemma}}*) unite (ListBag ((e,c+z):xs')) bagy
             = unite (ListBag ((inc (e,z) (e,c)):xs')) bagy
             (*\sEq{\ref{mapLemma}}*) unite (ListBag ((inc (e,z) x):(map (inc (e,z)) xs'))) bagy
             = unite (ListBag (map (inc (e,z)) (x:xs'))) bagy
             = unite (ListBag (map (inc (e,z)) xs)) bagy
             (*\sEq{A1}*) unite (add (e,z) (ListBag xs)) bagy
\end{code}
\end{proof}
\begin{comment}
%-------------------------------------------------------------------------------
\begin{lemma}{Associativity of \verb|unite|}
\begin{code}
unite (ListBag xs) (unite (ListBag ys) (ListBag zs))
          = unite (unite (ListBag xs) (ListBag ys)) (ListBag zs)
\end{code}
\end{lemma}
\begin{proof}by structural induction on xs\\
\verb|xs=[]|
\begin{code}
unite (ListBag xs) (unite (ListBag ys) (ListBag zs))
          = unite (ListBag []) (unite (ListBag ys) (ListBag zs))
          = unite (ListBag ys) (ListBag zs)
          = unite (unite (ListBag []) (ListBag ys)) (ListBag zs)
          = unite (unite (ListBag xs) (ListBag ys)) (ListBag zs)
\end{code}
\verb|xs=(x:xs')|
\begin{code}
unite (ListBag xs) (unite (ListBag ys) (ListBag zs))
          = unite (ListBag (x:xs')) (unite (ListBag ys) (ListBag zs))
          = unite (ListBag xs') (add x (unite (ListBag ys) (ListBag zs)))
          (*\sEq{\ref{addLemma}}*) unite (ListBag xs') (unite (add x (ListBag ys)) (ListBag zs))
          (*\sEq{IH}*) unite (unite (ListBag xs') (add x (ListBag ys))) (ListBag zs)
          = unite (unite (ListBag (x:xs')) (ListBag ys)) (ListBag zs)
          = unite (unite (ListBag xs) (ListBag ys)) (ListBag zs)
\end{code}
\end{proof}
\end{comment}
%-------------------------------------------------------------------------------
\begin{proof}of Claim \ref{bagClaim} by structural induction on xs\\
\verb|xs=[]|
\begin{code}
bag (xs++ys) = bag ([]++ys)
             = bag ys
             = unite (ListBag []) (bag ys) 
             = unite (bag []) (bag ys) 
             = unite (bag xs) (bag ys) 
\end{code}
\verb|xs=(x:xs')|
\begin{code}
bag (xs++ys) = bag ((x:xs')++ys)
             = bag (x:(xs'++ys))
             = add (x,1) (bag (xs'++ys))
             (*\sEq{IH}*) add (x,1) (unite (bag xs') (bag ys))
             (*\sEq{\ref{addLemma}}*) unite (add (x,1) (bag xs')) (bag ys)
             = unite (bag (x:xs')) (bag ys)
             = unite (bag xs) (bag ys)
\end{code}
\end{proof}