\section{foldl map}
\begin{code}
foldl :: (a -> b -> a) -> a -> [b] -> a
foldl f a []     = a
foldl f a (x:xs) = foldl f (f a x) xs
\end{code}
\begin{claim}\ 
\begin{code}
foldl f a.map g = foldl h a
          h b x = f b (g x)
\end{code}
\end{claim}
\begin{proof}we show the equivalent claim \\
\verb|foldl f a (map g xs) = foldl h a xs|\\
\verb|               h b x = f b (g x)|\\
by structural induction on xs\\
\verb|xs=[]|
\begin{code}
foldl f a (map g xs) = foldl f a (map g [])
                     = foldl f a []
                     = a
                     = foldl h a []
                     = foldl h a xs
\end{code}
\verb|xs=(x:xs')|
\begin{code}
foldl f a (map g xs) = foldl f a (map g (x:xs'))
                     = foldl f a ([g x]++(map g xs'))
                     = foldl f (f a (g x)) (map g xs')
                     (*\sEq{IH}*) foldl h (f a (g x)) xs'
                     = foldl h (h a x) xs'
                     = foldl h a (x:xs')
                     = foldl h a xs
\end{code}
\end{proof}