\section{map concat}
\verb|===|\\
\begin{code}
(.) :: (b -> c) -> (a -> b) -> a -> c
f . g = \x -> f (g x)
\end{code}
\begin{code}
concat :: [[a]] -> [a]
concat []     = []
concat (x:xs) = x++(concat xs)
\end{code}
\begin{code}
map :: (a -> b) -> [a] -> [b] 
map f []     = []
map f (x:xs) = [f x]++(map f xs)
\end{code}
\begin{claim}\ 
\begin{code}
map f.concat = concat.map (map f)
\end{code}
\end{claim}
\begin{proof}structural induction on xs\\
\verb|xs=[]|
\begin{code}
(map f.concat) xs = (map f.concat) []
                  = map f (concat [])
                  = map f []
                  = []
                  = concat []
                  = concat (map (map f) [])
                  = (concat.map (map f)) []
                  = (concat.map (map f)) xs
\end{code}
\verb|xs=(x:xs')|
structural induction on x\\
\verb|  x=[]|
\begin{code}
(map f.concat) xs = (map f.concat) (x:xs')
                  = map f (concat ([]:xs'))
                  = map f ([]++(concat xs'))
                  = map f (concat xs')
                  (*\sEq{IH}*) (concat.map (map f)) xs'
                  = concat (map (map f) xs')
                  = []++(concat (map (map f) xs'))
                  = concat [[]]++(map (map f) xs')
                  = concat [map f []]++(map (map f) xs')
                  = concat (map (map f) ([]:xs'))
                  = concat (map (map f) xs)
                  = (concat.map (map f)) xs
\end{code}
\verb|  x=(y:ys)|
\begin{code}
(map f.concat) xs = (map f.concat) (x:xs')
                  = map f (concat ((y:ys):xs'))
                  = map f ((y:ys)++(concat xs'))
                  = [f y]++(map f (ys++(concat xs')))
                  = [f y]++(map f (concat (ys:xs')))
                  (*\sEq{IH}*) [f y]++((concat.map (map f)) (ys:xs'))
                  = [f y]++(concat (map (map f) (ys:xs')))
                  = [f y]++(concat [map f ys]++(map (map f) xs'))
                  = [f y]++(map f ys)++(concat (map (map f) xs'))
                  = (map f (y:ys))++(concat (map (map f) xs'))
                  = concat [map f (y:ys)]++(map (map f) xs')
                  = concat (map (map f) ((y:ys):xs'))
                  = concat (map (map f) (x:xs'))
                  = concat (map (map f) xs)
                  = (concat.map (map f)) xs
\end{code}
\end{proof}
\newpage
alternative proof
\begin{proof} we show the equivalent claim \\
\verb|map f (concat xs) = concat (map (map f) xs)|\\
structural induction on xs\\
\verb|xs=[]|
\begin{code}
map f (concat xs) = map f (concat [])
                  = map f []
                  = []
                  = concat []
                  = concat (map (map f) [])
                  = concat (map (map f) xs)
\end{code}
\verb|xs=(x:xs')|
structural induction on x\\
\verb|  x=[]|
\begin{code}
map f (concat xs) = map f (concat ([]:xs'))
                  = map f ([]++(concat xs'))
                  = map f (concat xs')
                  (*\sEq{IH}*) concat (map (map f) xs')
                  = []++(concat (map (map f) xs'))
                  = concat [[]]++(map (map f) xs')
                  = concat [map f []]++(map (map f) xs')
                  = concat (map (map f) ([]:xs'))
                  = concat (map (map f) xs)
\end{code}
\verb|  x=(y:ys)|
\begin{code}
map f (concat xs) = map f (concat ((y:ys):xs'))
                  = map f ((y:ys)++(concat xs'))
                  = [f y]++(map f (ys++(concat xs')))
                  = [f y]++(map f (concat (ys:xs')))
                  (*\sEq{IH}*) [f y]++(concat (map (map f) (ys:xs')))
                  = [f y]++(concat [map f ys]++(map (map f) xs'))
                  = [f y]++(map f ys)++(concat (map (map f) xs'))
                  = (map f (y:ys))++(concat (map (map f) xs'))
                  = concat [map f (y:ys)]++(map (map f) xs')
                  = concat (map (map f) ((y:ys):xs'))
                  = concat (map (map f) xs)
\end{code}
\end{proof}